EvalE.v
@@ -1,38 +1,164 @@
+(** * Interpreters for the core langage *)
+(** Contains two implementations of interpreters with
+    different value envirionment representations *)
+Require Import Relations Morphisms.
 Require Import String.
 Require Import List.
 Require Import Ast.
 
 (* TODO: we use definition of monads from Template Coq,
    but (as actually comment in the [monad_utils] says, we
-   should use a real monad library. )*)
+   should use a real monad library) *)
 Require Import Template.monad_utils.
 
 
 Import ListNotations.
 Import MonadNotation.
 
-Module Interpreter.
+(* Common definitions *)
 
-  Definition env A := list (string * A).
+Inductive res A :=
+| Ok : A -> res A
+| NotEnoughFuel : res A
+| EvalError : string -> res A.
 
-  Definition lookup {A : Type} (ρ : env A) (key : string) : option A :=
-    option_map snd (List.find (fun '(key',v) => if (string_dec key key')
-                          then Coq.Init.Datatypes.true else Coq.Init.Datatypes.false) ρ).
 
-  Notation "ρ # '(' k ')'" := (lookup ρ k) (at level 10).
-  (** A value environment extension: *)
-  Notation "E # [ k ~> v ]" := ((k,v) :: E) (at level 50).
+Arguments Ok {_}.
+Arguments NotEnoughFuel {_}.
+Arguments EvalError {_}.
 
+Instance res_monad : Monad res :=
+  { ret := @Ok;
+    bind := fun _ _ r f => match r with
+                    | Ok v => f v
+                    | EvalError msg => EvalError msg
+                    | NotEnoughFuel => NotEnoughFuel
+                        end }.
+
+Definition res_map {A B} (f : A -> B) (r : res A) : res B :=
+  v <- r ;;
+  ret (f v).
+
+Definition option_to_res {A : Type} (o : option A) (msg : string) :=
+  match o with
+  | Some v => Ok v
+  | None => EvalError msg
+  end.
+
+Definition todo {A} := EvalError (A:=A) "Not implemented".
+
+Module InterpreterEnvList.
+
+  (* An interpreter that uses list-like structure to represent environments.
+     Currently does not handle recursion [fix] *)
+
+  (* Inspired by this: https://www.cs.bgu.ac.il/~elhadad/advpro/course6.html *)
+  Inductive env (A : Type) :=
+  | enEmpty  : env A
+  | enCons   : name -> A -> env A -> env A
+  | enRec    : name -> name -> expr -> type -> type -> env A -> env A.
+
+  Arguments enEmpty {_}.
+  Arguments enCons {_}.
+  Arguments enRec {_}.
+
+  Fixpoint concat_env {A : Type} (ρ ρ' : env A) :=
+    match ρ with
+    | enEmpty => ρ'
+    | enCons nm v ρ'' => enCons nm v (concat_env ρ'' ρ')
+    | enRec fixname nm e ty1 ty2 ρ'' => enRec fixname nm e ty1 ty2 (concat_env ρ'' ρ')
+    end.
+
+  Fixpoint list_to_env {A : Type} (xs : list (name * A)) : env A :=
+    match xs with
+    | [] => enEmpty
+    | (k,v) :: xs' => enCons k v (list_to_env xs')
+    end.
 
   Inductive val : Type :=
   | vConstr : inductive -> name -> list val -> val
   | vClos   : env val -> name ->
-              type (*types are used to convert closures back to lambdas *) ->
+              type ->(* types are used to convert closures back to lambdas *)
               expr -> val.
+
+  Inductive ForallEnv {A} (P : A -> Prop) : env A -> Prop :=
+  | feNil : ForallEnv P enEmpty
+  | feCons : forall (nm : name) (a : A) (ρ : env A), P a -> ForallEnv P ρ -> ForallEnv P (enCons nm a ρ)
+  | feRec  : forall fixname nm e ty1 ty2 ρ,
+      ForallEnv P ρ -> ForallEnv P (enRec fixname nm e ty1 ty2 ρ).
+
+
+  (* An induction principle that takes into account nested occurences of elements of [val]
+     in the list of arguments of [vConstr] and in the environment of [vClos] *)
+  Definition val_ind_full
+     (P : val -> Prop)
+     (Hconstr : forall (i : inductive) (n : name) (l : list val), Forall P l -> P (vConstr i n l))
+     (Hclos : forall (ρ : env val) (n : name) (ty : type) (e0 : expr),
+          ForallEnv P ρ -> P (vClos ρ n ty e0)) :
+    forall v : val, P v.
+    refine (fix val_ind_fix (v : val) := _).
+    destruct v.
+    + apply Hconstr.
+      induction l. constructor. constructor. apply val_ind_fix. apply IHl.
+    + apply Hclos.
+      induction e.
+      * constructor.
+      * constructor. apply val_ind_fix. apply IHe.
+      * constructor. apply IHe.
+  Defined.
+
+  (* For some reason, this is not a part of the standard lib *)
+  Lemma Forall_app {A} (l1 l2 : list A) P :
+    Forall P (l1 ++ l2) <-> Forall P l1 /\ Forall P l2.
+  Proof.
+    split.
+    - intros H. induction l1.
+      + simpl in *. easy.
+      + simpl in *. inversion H. subst.
+        split.
+        * constructor. assumption.
+          destruct (IHl1 H3). assumption.
+        * destruct (IHl1 H3). assumption.
+    - intros H. induction l1.
+      + simpl in *. easy.
+      + simpl in *. destruct H as [H1 H2].
+        constructor;inversion H1;auto.
+  Qed.
+
+  Lemma Forall_rev {A} {l : list A} P : Forall P l -> Forall P (rev l).
+  Proof.
+    intros H.
+    induction l.
+    + constructor.
+    + simpl. apply Forall_app.
+      inversion H;auto.
+  Qed.
+
+  Fixpoint lookup (ρ : env val) (key : string) : option val :=
+    match ρ with
+    | enEmpty => None
+    | enCons nm a ρ' =>
+      if (nm =? key) then Some a else lookup ρ' key
+    | enRec fixname nm e ty1 ty2 ρ' =>
+      if (fixname =? key) then Some (vClos ρ nm ty1 e) else lookup ρ' key
+    end.
+
+  Notation "ρ # '(' k ')'" := (lookup ρ k) (at level 10).
+  (** A value environment extension: *)
+  Notation "ρ # [ k ~> v ]" := (enCons k v ρ) (at level 50).
+
+  Fixpoint remove_by_key  (key : name) (ρ : env val) : env val :=
+    match ρ with
+      | enEmpty => enEmpty
+      | enCons nm a ρ' => if (nm =? key) then remove_by_key key ρ'
+                           else enCons nm a (remove_by_key key ρ')
+      | enRec fixname nm e ty1 ty2 ρ'=> if (fixname =? key) then remove_by_key key ρ'
+                          else enRec fixname nm e ty1 ty2 (remove_by_key key ρ')
+    end.
 
   (* This doesn't work for the same reason as for STLC: in the case
      for application we don't know if [b] is decreasing.
-     Alhough, for the relational specification we can prove this using logical relations *)
+     Although, for the relational specification we can prove this using logical relations *)
   Fail Fixpoint expr_eval (ρ : env val) (e : expr) {struct e} : option val :=
       match e with
       | eRel i => None
@@ -66,31 +192,6 @@ Module Interpreter.
       | eFix nm ty b => None
       end.
 
-  Inductive res A :=
-  | Ok : A -> res A
-  | NotEnoughFuel : res A
-  | EvalError : string -> res A.
-
-
-  Arguments Ok {_}.
-  Arguments NotEnoughFuel {_}.
-  Arguments EvalError {_}.
-
-  Instance res_monad : Monad res :=
-    { ret := @Ok;
-      bind := fun _ _ r f => match r with
-                      | Ok v => f v
-                      | EvalError msg => EvalError msg
-                      | NotEnoughFuel => NotEnoughFuel
-                      end }.
-
-  Definition option_to_res {A : Type} (o : option A) (msg : string) :=
-    match o with
-    | Some v => Ok v
-    | None => EvalError msg
-    end.
-
-  Definition todo {A} := EvalError (A:=A) "Not implemented".
 
   Definition ind_name (v : val) :=
     match v with
@@ -98,7 +199,6 @@ Module Interpreter.
     | _ => None
     end.
 
-  (* FIXME: should be extended to match the arguments of the constructor *)
   Fixpoint match_pat {A} (constr_name : name) (constr_args : list A) (bs : list (pat * expr)) :=
     match bs with
     | [] => None
@@ -116,7 +216,7 @@ Module Interpreter.
     | S n =>
       match e with
       | eRel i => EvalError "Indices as variables are not supported"
-      | eVar nm => option_to_res (ρ # (nm)) ("Var not found: " ++ nm)
+      | eVar nm => option_to_res (ρ # (nm)) (nm ++ " - var not found")
       | eLambda nm ty b =>
         Ok (vClos ρ nm ty b)
       | eLetIn nm e1 ty e2 => todo
@@ -139,7 +239,8 @@ Module Interpreter.
         match (expr_eval n Σ ρ e) with
         | Ok (vConstr ind' c vs) => if (string_dec ind ind') then
                                       match (match_pat c vs bs) with
-                                      | Some (var_assign, v) => expr_eval n Σ (List.app ρ var_assign) v
+                                      | Some (var_assign, v) =>
+                                        expr_eval n Σ (concat_env (list_to_env var_assign) ρ) v
                                       | None => EvalError "No such constructor"
                                       end
                                     else EvalError ("Expecting inductive " ++ ind ++
@@ -147,66 +248,234 @@ Module Interpreter.
         | v => v
         end
       | eFix fixname vn ty1 ty2 b as e =>
-        let lam := eLambda vn ty1 b in
-        (* ρ below should be be extended recursively as well :( *)
-        match (expr_eval n Σ ρ lam) with
-        | Ok v' => Ok (vClos (ρ # [fixname ~> v']) vn ty1 b )
-        | e => e
-        end
-         (* expr_eval n Σ (ρ # [fixname ~> vClos ρ fixname (tyArr ty1 ty2) e ]) b *)
+        expr_eval n Σ (enRec fixname vn b ty1 ty2 ρ) (eLambda vn ty1 b)
       end
     end.
 
-  Definition fun_env A := name -> A.
-  Inductive fval : Type :=
-  | fvConstr : inductive -> name -> list fval -> fval
-  | fvClos   : fun_env fval -> name ->
-              type (*types are used to convert closures back to lambdas *) ->
-              expr -> fval.
+  Definition map_env {A B : Type} (f : A -> B) : env A -> env B :=
+    fix menv (ρ : env A) :=
+      match ρ with
+      | enEmpty => enEmpty
+      | enCons nm v ρ' => enCons nm (f v) (menv ρ')
+      | enRec fixname nm e ty1 ty2 ρ' => enRec fixname nm e ty1 ty2 (menv ρ')
+      end.
 
-  Definition ext_env (ρ : fun_env fval) (k : name) v := fun k' => if (string_dec k k') then v else ρ k'.
-  Fixpoint ext_env_list (ρ : fun_env fval) (kvs : list (name * fval)) :=
-    match kvs with
-    | [] => ρ
-    | (k,v) :: kvs' => ext_env (ext_env_list ρ kvs' ) k v
+  Fixpoint env_to_list {A : Type} (ρ : env A) : list (name * A) :=
+    match ρ with
+    | enEmpty => []
+    | enCons nm v ρ' => (nm, v) :: env_to_list ρ'
+    | enRec fixname nm e ty1 ty2 ρ' => env_to_list ρ'
+    end.
+
+  (* This is equivalent to the composition env_to_list ∘ (map_env f), but
+     we if we use the comosition in the definition of from_val, then Coq cannot
+     recognise it as a fixpoint. So, we have to merge the two definitions *)
+  Definition map_env_list {A B : Type} (f : A -> B) : env A -> list (name * B) :=
+    fix menv (ρ : env A) :=
+      match ρ with
+      | enEmpty => []
+      | enCons nm v ρ' => (nm, f v) :: (menv ρ')
+      | enRec fixname nm e ty1 ty2 ρ' => menv ρ'
+      end.
+
+
+  Definition lookup_list {A : Type} (ρ : list (name * A)) (key : string) : option A :=
+    option_map snd (List.find (fun '(key',v) => if (string_dec key key')
+                          then Coq.Init.Datatypes.true else Coq.Init.Datatypes.false) ρ).
+
+  Fixpoint remove_by_key_list (key : name) (ρ : list (name * expr)) : list (name * expr) :=
+    match ρ with
+      | [] => []
+      | (nm,a) :: ρ' => if (nm =? key) then remove_by_key_list key ρ'
+                           else (nm, a) :: (remove_by_key_list key ρ')
     end.
 
 
-  Definition default_fun_env : fun_env fval := fun _ => fvConstr "Error" "Error" [].
-  Definition pfun_env A := name -> res A.
+    (* NOTE: assumes, that [e] is a closed expression! *)
+ Fixpoint subst_env (ρ : list (name * expr)) (e : expr) : expr :=
+  match e with
+  | eRel i as e' => e'
+  | eVar nm  => match lookup_list ρ nm with
+                    | Some v => v
+                    | None => e
+                    end
+  | eLambda nm ty b => eLambda nm ty (subst_env (remove_by_key_list nm ρ) b)
+  | eLetIn nm e1 ty e2 => eLetIn nm (subst_env ρ e1) ty (subst_env (remove_by_key_list nm ρ) e2)
+  | eApp e1 e2 => eApp (subst_env ρ e1) (subst_env ρ e2)
+  | eConstr t i as e' => e'
+  | eConst nm => eConst nm
+  | eCase nm_i ty e bs =>
+    (* TODO: this case is not complete! We ignore variables bound by patterns *)
+    eCase nm_i ty (subst_env ρ e) (map (fun x => (fst x, subst_env ρ (snd x))) bs)
+  | eFix nm v ty1 ty2 b => eFix nm v ty1 ty2 (subst_env (remove_by_key_list v ρ) b)
+  end.
 
-  Definition penv_to_total ρ : fun_env fval :=
-    fun k =>
-    match ρ k with
-    | Ok v => v
-    | EvalError msg => fvConstr msg "Error" []
-    | NotEnoughFuel => fvConstr "Not enough fuel" "Error" []
+  (* Converting from values back to expression.
+     This will be used to compare results of the evaluation with different semantics, or
+     for stating soundness theorem for the translation to a different language, e.g.
+     to Template Coq terms.
+
+     The most non-trival part is to convert closures, for which we have to perform some form
+     of subsitution of values from the value environment (see [subst_env])
+     Inspired by the implementation of
+     "A Certified Implementation of ML with Structural Polymorphism" by Jacques Garrigue.
+   *)
+  Fixpoint from_val (v : val) : expr :=
+    match v with
+    | vConstr x i vs => vars_to_apps (eConstr x i) (map from_val vs)
+    | vClos ρ nm ty e =>
+      match ρ with
+      | enRec fixname _ _ ty1 ty2 _ =>
+        subst_env (map_env_list from_val ρ) (eFix fixname nm ty ty2 e)
+      | _ => subst_env (map_env_list from_val ρ) (eLambda nm ty e)
+      end
+    end.
+
+  Definition inst_env (ρ : env val) (e : expr) : expr := subst_env (map_env_list from_val ρ) e.
+
+  Reserved Notation "v1 ≈ v2" (at level 50).
+
+  Inductive val_equiv : relation val :=
+  | veqConstr i n (vs1 vs2 : list val) :
+      Forall2 (fun v1 v2 => v1 ≈ v2) vs1 vs2 -> vConstr i n vs1 ≈ vConstr i n vs2
+  | veqClos ρ1 ρ2 nm ty e1 e2 :
+      inst_env ρ1 (eLambda nm ty e1) = inst_env ρ2 (eLambda nm ty e2) ->
+      vClos ρ1 nm ty e1 ≈ vClos ρ2 nm ty e2
+  where
+  "v1 ≈ v2" := (val_equiv v1 v2).
+
+  Definition list_val_equiv vs1 vs2 := Forall2 (fun v1 v2 => v1 ≈ v2) vs1 vs2.
+  Notation " vs1 ≈ₗ vs2 " := (list_val_equiv vs1 vs2) (at level 50).
+
+  Instance val_equiv_reflexive : Reflexive val_equiv.
+  Proof.
+    intros v. induction v using val_ind_full.
+    + constructor.
+      induction l;constructor; inversion H; easy.
+    + constructor;reflexivity.
+  Defined.
+
+  (* TODO:  Add the rest to prove that [val_equiv] is indeed an equivalence *)
+  Axiom val_equiv_symmetric : Symmetric val_equiv.
+  Axiom val_equiv_transitive : Transitive val_equiv.
+
+  Existing Instance val_equiv_symmetric.
+  Existing Instance val_equiv_transitive.
+
+  Add Relation val val_equiv
+      reflexivity proved by val_equiv_reflexive
+      symmetry proved by val_equiv_symmetric
+      transitivity proved by val_equiv_transitive as val_equiv_rel.
+
+  (* TODO:  Define these  *)
+  Axiom list_val_equiv_reflexive : Reflexive list_val_equiv.
+  Axiom list_val_equiv_symmetric : Symmetric list_val_equiv.
+  Axiom list_val_equiv_transitive : Transitive list_val_equiv.
+
+  Existing Instance list_val_equiv_symmetric.
+  Existing Instance list_val_equiv_symmetric.
+  Existing Instance list_val_equiv_transitive.
+
+  Add Relation (list val) list_val_equiv
+      reflexivity proved by list_val_equiv_reflexive
+      symmetry proved by list_val_equiv_symmetric
+      transitivity proved by list_val_equiv_transitive as list_val_equiv_rel.
+
+  Lemma list_val_compat v1 v2 vs1 vs2 :
+    v1 ≈ v2 -> vs1 ≈ₗ vs2 -> (v1 :: vs1) ≈ₗ (v2 :: vs2).
+  Proof.
+    intros Heq Heql.
+    constructor;easy.
+  Qed.
+
+  Instance cons_compat : Proper (val_equiv ==> list_val_equiv ==> list_val_equiv) cons.
+  Proof.
+    cbv;intros;apply list_val_compat;assumption.
+  Defined.
+
+  Lemma constr_cons_compat (vs1 vs2 : list val) (i : inductive) (nm : name) :
+    vs1 ≈ₗ vs2 -> (vConstr i nm vs1) ≈ (vConstr i nm vs2).
+  Proof.
+    intros Heql.
+    constructor.
+    induction Heql.
+    + constructor.
+    + constructor; assumption.
+  Defined.
+
+  Instance constr_morph i nm : Proper (list_val_equiv ==> val_equiv) (vConstr i nm).
+  Proof.
+    cbv;intros;apply constr_cons_compat;assumption.
+  Defined.
+
+End InterpreterEnvList.
+
+Module InterpreterEnvFun.
+
+  (* An interpreter that uses functions to represent environments.
+     Moreover, we need partial environments, because recursive environment extension
+     might not terminate *)
+  Definition env A := name -> res A.
+  Definition default_fun_env {A : Type}: env A :=
+    fun k => EvalError ("Undefined var :" ++ k).
+  Definition in_env {A} k (ρ : env A) := exists v, ρ k = Ok v.
+
+  Definition remove_by_key {A : Type} (key : string) (ρ : InterpreterEnvFun.env A)
+  : InterpreterEnvFun.env A :=
+  fun key' => if (eqb key key') then (default_fun_env key)
+           else ρ key.
+
+  Lemma remove_spec {A} k (ρ : env A) : ~ in_env k (remove_by_key k ρ).
+  Proof.
+    intros H. unfold in_env,remove_by_key in H.
+    destruct H.
+    rewrite eqb_refl in H.
+    inversion H.
+  Qed.
+
+
+  Inductive val : Type :=
+  | vConstr : inductive -> name -> list val -> val
+  | vClos   : env val -> name ->
+               type (* types are used to convert closures back to lambdas *) ->
+               expr -> val.
+
+  Definition ext_env (ρ : env val) (k : name) v :=
+    fun k' => if (string_dec k k') then v else ρ k'.
+
+  (* Notation "ρ # '(' k ')'" := (ρ k) (at level 10). *)
+  (** A value environment extension: *)
+  Notation "ρ # [ k ~> v ]" := (ext_env ρ k v) (at level 50).
+
+  Fixpoint ext_env_list (ρ : env val) (kvs : list (name * val)) :=
+    match kvs with
+    | [] => ρ
+    | (k,v) :: kvs' => ext_env (ext_env_list ρ kvs' ) k (Ok v)
     end.
 
   Definition ext_env_rec (fixname : name) (var : name) (ty : type) (e : expr)
-             (ρ : fun_env fval) :=
-    fix rec_enc fuel : res (pfun_env fval) :=
+             (ρ : env val) :=
+    fix rec_enc fuel : res (env val) :=
         match fuel with
         | O => NotEnoughFuel
         | S n => Ok (fun k =>
                       if (eqb fixname k) then
                         match rec_enc n with
-                          (* FIXME: [penv_to_total] is a hack*)
-                        | Ok ρ' => Ok (fvClos (penv_to_total ρ') var ty e)
+                        | Ok ρ' => Ok (vClos ρ' var ty e)
                         | EvalError msg => EvalError msg
                         | NotEnoughFuel => NotEnoughFuel
                         end
-                      else Ok (ρ k))
+                      else ρ k)
         end.
 
   (* This is a simple fact, but it shows that we have two sources of partiality:
-     possible non-termination of the recursive xontext extension and a corresoinding
-     lookup operation (here it is just a function application, but it retirnes a
-     value of type [res fvar] instead of plain [fvar] ) *)
+     possible non-termination of the recursive context extension and a corresponding
+     lookup operation (here it is just a function application, but it returns a
+     value of type [res fvar] instead of a plain [fvar] ) *)
   Lemma ext_env_rec_extend_lookup : forall n nm vn ty e ρ ρ',
-      ext_env_rec nm vn ty e (penv_to_total ρ) n = Ok ρ ->
+      ext_env_rec nm vn ty e ρ n = Ok ρ ->
       ρ nm = Ok ρ' ->
-    exists ρ'', ρ' = fvClos ρ'' vn ty e.
+    exists ρ'', ρ' = vClos ρ'' vn ty e.
   Proof.
     intros n nm nv ty e ρ ρ' H1 H2. destruct n.
     + inversion H1.
@@ -216,61 +485,88 @@ Module Interpreter.
       * inversion H1 as [H3]. simpl in *.
         rewrite <- H3 in H2.
         rewrite eqb_refl in H2.
+        inversion H2. subst.
         eexists.
-        inversion_clear H2. f_equal.
+        inversion_clear H2. f_equal. reflexivity.
   Qed.
 
   Import Basics.
 
   Open Scope program_scope.
 
-  Fixpoint expr_eval_fun (fuel : nat) (Σ : global_env) (ρ : fun_env fval) (e : expr) : res fval :=
+  Fixpoint expr_eval (fuel : nat) (Σ : global_env) (ρ : env val) (e : expr) : res val :=
     match fuel with
     | O => NotEnoughFuel
     | S n =>
       match e with
       | eRel i => EvalError "Indices as variables are not supported"
-      | eVar nm => Ok (ρ nm)
-      | eLambda nm ty b =>
-        Ok (fvClos ρ nm ty b)
-      | eLetIn nm e1 ty e2 => todo
+      | eVar nm => ρ nm
+      | eLambda nm ty b => ret (vClos ρ nm ty b)
+      | eLetIn nm e1 ty e2 =>
+        expr_eval n Σ (ρ # [nm ~> (expr_eval n Σ ρ e1)]) e2
       | eApp e1 e2 =>
-        match (expr_eval_fun n Σ ρ e1), (expr_eval_fun n Σ ρ e2) with
-        | Ok (fvClos ρ' nm _ b), Ok v =>
-          match (expr_eval_fun n Σ (ext_env ρ' nm v) b) with
-          | Ok v' => Ok v'
-          | err => err
-          end
-        | Ok (fvConstr ind n vs), Ok v => Ok (fvConstr ind n (List.app vs [v]))
-        | EvalError msg, _ => EvalError msg
-        | _, EvalError msg => EvalError msg
-        | NotEnoughFuel,_ | _, NotEnoughFuel => NotEnoughFuel
+        v1 <- expr_eval n Σ ρ e1 ;;
+        v2 <- expr_eval n Σ ρ e2 ;;
+        match v1 with
+        | vClos ρ' nm _ b =>
+          expr_eval n Σ (ρ' # [nm ~> ret v2]) b
+        | vConstr ind n vs => ret (vConstr ind n (List.app vs [v2]))
         end
       | eConstr t i =>
-        Ok (fvConstr t i [])
+        Ok (vConstr t i [])
       | eConst nm => todo
+        (* option_to_res (lookup_global Σ nm) ("Constant " ++ nm ++ " not found") *)
       | eCase (ind,i) ty e bs =>
-        match (expr_eval_fun n Σ ρ e) with
-        | Ok (fvConstr ind' c vs) => if (string_dec ind ind') then
-                                      match (match_pat c vs bs) with
-                                      | Some (var_assign, v) =>
-                                        expr_eval_fun n Σ (ext_env_list ρ var_assign) v
-                                      | None => EvalError "No such constructor"
-                                      end
-                                    else EvalError ("Expecting inductive " ++ ind ++
-                                                     " but found " ++ ind')
-        | v => v
+        v <- (expr_eval n Σ ρ e);;
+        match v with
+        | vConstr ind' c vs =>
+          if (string_dec ind ind') then
+            (* The pattern-mathcing is the same for the both interpreters,
+               so we just reuse it *)
+            match (InterpreterEnvList.match_pat c vs bs) with
+            | Some (var_assign, v) =>
+              expr_eval n Σ (ext_env_list ρ var_assign) v
+            | None =>
+              EvalError ("No such constructor for inductive " ++ ind)
+            end
+          else EvalError ("Expecting inductive " ++ ind ++ " but found " ++ ind')
+        | _ => EvalError "Not a constructor"
         end
       | eFix fixname vn ty1 ty2 e =>
-        match (ext_env_rec fixname vn ty1 e ρ n) with
-        | Ok ρ' => expr_eval_fun n Σ (penv_to_total ρ') (eLambda vn ty1 e)
-        | EvalError msg => EvalError msg
-        | NotEnoughFuel => NotEnoughFuel
-        end
+        ρ' <- ext_env_rec fixname vn ty1 e ρ n ;;
+        expr_eval n Σ ρ' (eLambda vn ty1 e)
       end
     end.
 
+  Fixpoint subst_env (ρ : InterpreterEnvFun.env expr) (e : expr) : expr :=
+  match e with
+  | eRel i as e' => e'
+  | eVar nm  => match ρ nm with
+                    | Ok v => v
+                    | _ => e
+                    end
+  | eLambda nm ty b => eLambda nm ty (subst_env (remove_by_key nm ρ) b)
+  | eLetIn nm e1 ty e2 => eLetIn nm (subst_env ρ e1) ty (subst_env (remove_by_key nm ρ) e2)
+  | eApp e1 e2 => eApp (subst_env ρ e1) (subst_env ρ e2)
+  | eConstr t i as e' => e'
+  | eConst nm => eConst nm
+  | eCase nm_i ty e bs =>
+    (* TODO: this case is not complete! We ignore variables bound by patterns *)
+    eCase nm_i ty (subst_env ρ e) (map (fun x => (fst x, subst_env ρ (snd x))) bs)
+  | eFix nm v ty1 ty2 b => eFix nm v ty1 ty2 (subst_env (remove_by_key v ρ) b)
+  end.
 
+
+  (* Cannot make Coq to recognize this as a valid fixpoint *)
+  Fail Fixpoint from_val (v : val) {struct v} : expr :=
+    match v with
+    | vConstr x i vs => vars_to_apps (eConstr x i) (map from_val vs)
+    | vClos ρ nm ty e =>
+      subst_env (fun k => v <- ρ k ;; ret (from_val v)) (eLambda nm ty e)
+    end.
+End InterpreterEnvFun.
+
+Module Examples.
   Import BaseTypes.
   Import StdLib.
 
@@ -283,7 +579,10 @@ Module Interpreter.
      |].
 
   Example eval_prog1 :
-    expr_eval 3 Σ [] prog1 = Ok (vConstr "Coq.Init.Datatypes.bool" "false" []).
+    InterpreterEnvList.expr_eval 3 Σ InterpreterEnvList.enEmpty prog1 = Ok (InterpreterEnvList.vConstr "Coq.Init.Datatypes.bool" "false" []).
   Proof. simpl. reflexivity. Qed.
 
-End Interpreter.
+  Example eval_prog1' :
+    InterpreterEnvFun.expr_eval 3 Σ InterpreterEnvFun.default_fun_env  prog1 = Ok (InterpreterEnvFun.vConstr "Coq.Init.Datatypes.bool" "false" []).
+  Proof. simpl. reflexivity. Qed.
+End Examples.
