Correctness.v
@@ -1,0 +1,30 @@
+(* Proof of correctness of the translation from core language expression to the Template Coq terms *)
+Require Import Ast EvalE Facts CustomTactics String.
+Require Template.WcbvEval.
+Require Import Template.All.
+
+Require Import List.
+
+Import ListNotations.
+
+Notation "Σ ;;; Γ |- t1 ⇓ t2 " := (WcbvEval.eval Σ Γ t1 t2) (at level 50).
+Notation "T⟦ e ⟧ Σ " := (expr_to_term Σ e) (at level 40).
+
+Import InterpreterEnvList.
+
+Theorem expr_to_term_sound n ns ρ Σ1 Σ2 (Γ := []) (e : expr) (t : term) (v : val) :
+  Σ2 ;;; Γ |- T⟦indexify ns e⟧Σ1 ⇓ t ->
+  expr_eval n Σ1 ρ e = Ok v ->
+  t = T⟦from_val v⟧Σ1.
+Proof.
+  induction e using expr_ind_case.
+  + (* eRel - since we expect only named variables, this case is trivial*)
+    intros HT He. simpl in *. destruct n; tryfalse.
+  + (* eVar *)
+    intros HT He. destruct n; tryfalse. simpl in *.
+    (* we need to relate [ρ] and [ns] *)
+    admit.
+  + (* eLambda *)
+    intros HT He. destruct n; tryfalse. simpl in HT. simpl in He.
+    inversion He. simpl. inversion HT. subst.
+Admitted.
