CustomTactics.v
@@ -1,0 +1,35 @@
+(* A place for various tactic used for the development*)
+
+
+
+(* Tactics taken from the Software Foundations' LibTactics.v *)
+(* ================================================================= *)
+(** ** Absurd Goals *)
+
+(** [false_goal] replaces any goal by the goal [False].
+    Contrary to the tactic [false] (below), it does not try to do
+    anything else *)
+
+Tactic Notation "false_goal" :=
+  elimtype False.
+
+(** [false_post] is the underlying tactic used to prove goals
+    of the form [False]. In the default implementation, it proves
+    the goal if the context contains [False] or an hypothesis of the
+    form [C x1 .. xN  =  D y1 .. yM], or if the [congruence] tactic
+    finds a proof of [x <> x] for some [x]. *)
+
+Ltac false_post :=
+  solve [ assumption | discriminate | congruence ].
+
+(** [false] replaces any goal by the goal [False], and calls [false_post] *)
+
+Tactic Notation "false" :=
+  false_goal; try false_post.
+
+(** [tryfalse] tries to solve a goal by contradiction, and leaves
+    the goal unchanged if it cannot solve it.
+    It is equivalent to [try solve \[ false \]]. *)
+
+Tactic Notation "tryfalse" :=
+  try solve [ false ].
