Facts.v
@@ -1,0 +1,120 @@
+(* Various auxillary facts usefull for proving correctness of the translation and the interpreter *)
+
+Require Import CustomTactics.
+Require Import Ast.
+Require Import EvalE.
+Require Import String List.
+
+Require Import Morphisms Setoid.
+
+Require Import Template.monad_utils.
+
+Import FunctionalExtensionality.
+
+Open Scope string_scope.
+Import ListNotations.
+
+Import InterpreterEnvList.
+
+
+Section Values.
+
+  Lemma vars_to_apps_unfold vs : forall acc v,
+    vars_to_apps acc (vs ++ [v]) = eApp (vars_to_apps acc vs) v.
+  Proof.
+    simpl.
+    induction vs using rev_ind;intros acc v.
+    + reflexivity.
+    + simpl.
+      unfold vars_to_apps.
+      rewrite fold_left_app; easy.
+  Qed.
+
+  Lemma subst_env_empty :
+    forall e : expr, e = subst_env [] e.
+  Proof.
+    intros e.
+    induction e using expr_ind_case; simpl; try easy; try congruence.
+    f_equal;auto.
+    rewrite <- map_id at 1.
+    eapply @Induction.forall_map_spec.
+    eapply H.
+    intros x f. destruct x;simpl in *. f_equal. assumption.
+  Qed.
+
+  (* For simplicity, we consider only constructors of arity 0 and 1 *)
+  Inductive accepted_val : val -> Prop :=
+  | avContsr0 : forall i nm v, accepted_val v -> accepted_val (vConstr i nm [])
+  | avContsr1 : forall i nm v, accepted_val v -> accepted_val (vConstr i nm [v])
+  | avClos : forall ρ nm ty e, accepted_val (vClos ρ nm ty e).
+
+  Lemma expr_eval_econstr {n nm Σ ρ i v} :
+    expr_eval n Σ ρ (eConstr i nm) = Ok v ->
+    v = vConstr i nm [].
+  Proof.
+    intros H.
+    destruct n;inversion H. reflexivity.
+  Qed.
+
+  (** Correctness of the value-back-to-expression transformation *)
+  (* A a creterion of correctness we consider the property that
+     if we start with a value [v1], the output of [from_val v1] after evaluation,
+     should give as some [v2] equivalent to [v1].
+     Note that we cannot ask [v1] and [v2] to be equal,
+     instead we ask for equivalence. This is due to substitutions of the
+     values in the environment while converting closures back to expressions *)
+  Lemma from_val_correct n Σ v1 v2 :
+    accepted_val v1 ->
+    expr_eval n Σ enEmpty (from_val v1) = Ok v2 ->
+    v1 ≈ v2.
+  Proof.
+    intros Hav He.
+    revert dependent n.
+    revert dependent v2.
+    induction v1 using val_ind_full;intros v2 n0 H1.
+    + destruct n0;tryfalse.
+      inversion Hav;subst.
+      * simpl in H1. inversion H1. reflexivity.
+      * simpl in H1.
+        remember (expr_eval n0 Σ enEmpty (eConstr i n)) as c.
+        remember (expr_eval n0 Σ enEmpty (from_val v)) as fv.
+        destruct c as [c0 | | ];try destruct c0;destruct fv;tryfalse.
+        ** inversion H1 as [H1'].
+           symmetry in Heqfv.
+           apply Forall_inv in H.
+           pose proof (H H2 _ _ Heqfv) as HH. subst.
+           symmetry in Heqc.
+           pose proof (expr_eval_econstr Heqc) as HH1. inversion HH1;subst.
+           simpl. clear H Heqfv H1.
+           (* this rewrite actually uses setoid_rewrite along the ≈ relation *)
+           rewrite HH.
+           reflexivity.
+        ** symmetry in Heqc.
+           pose proof (expr_eval_econstr Heqc);tryfalse.
+    + simpl in H1.
+      destruct H.
+      * destruct n0;tryfalse. simpl in H1.
+        inversion_clear H1.
+        rewrite <- subst_env_empty. reflexivity.
+      * destruct n0;tryfalse. simpl in H1.
+        inversion_clear H1.
+        constructor.
+        destruct (nm =? n) eqn:Hnm.
+        ** unfold inst_env. simpl.
+           rewrite <- subst_env_empty.
+           apply eqb_eq in Hnm. subst.
+           rewrite eqb_refl. reflexivity.
+        ** unfold inst_env. simpl.
+           rewrite Hnm.
+           rewrite <- subst_env_empty.
+           reflexivity.
+      * (* It takes 2 steps to evaluate a fixpoint to a closure *)
+        destruct n0;tryfalse.
+        destruct n0;tryfalse. simpl in H1. inversion H1.
+        constructor.
+        unfold inst_env. simpl.
+        rewrite <- subst_env_empty.
+        reflexivity.
+  Qed.
+
+End Values.
